coq/theories/Env.v
@@ -1,0 +1,22 @@
+Require Import Coq.Classes.EquivDec.
+Require Import Coq.Lists.List.
+Import List.ListNotations.
+
+Set Implicit Arguments.
+Section Env.
+  Variable (K V: Type).
+  Context `{K_eq_dec: EquivDec.EqDec K eq}.
+  Definition t := list (K * V).
+  Definition emp: t := [].
+  Definition bind (k: K) (v: V) (e: t) : t :=
+    (k, v) :: e.
+  Fixpoint find (k: K) (e: t) : option V :=
+    match e with
+    | [] => None
+    | (k', v) :: s =>
+      if k == k'
+      then Some v
+      else find k s
+    end.
+End Env.
+Check find.
